Sketch state relation and eval correctness

pancake/proofs/pan_globalsProofScript.sml
@@ -11,6 +11,72 @@ val _ = set_grammar_ancestry  ["panSem", "pan_globals", "panProps", "panLang"];
 
 val s = ``s:('a,'ffi) panSem$state``
 
+Definition state_rel_def:
+  state_rel ctxt s t ⇔
+  s.top_addr = t.top_addr - ctxt.globals_size ∧
+  s.locals = t.locals ∧
+  s.base_addr = t.base_addr ∧
+  (∀v val.
+     FLOOKUP s.globals v = SOME val ⇒
+     ∃addr. FLOOKUP ctxt.globals v = SOME(shape_of val, addr) ∧
+            mem_load (shape_of val) (t.top_addr - addr) t.memaddrs t.memory = SOME val
+  ) ∧
+  s.memaddrs ⊆ t.memaddrs
+End
+
+Theorem compile_exp_correct:
+  ∀s e v ctxt t.
+  state_rel ctxt s t ∧
+  eval s e = SOME v
+  ⇒
+  eval t (compile_exp ctxt e) = SOME v
+Proof
+  recInduct eval_ind >> rpt strip_tac
+  >~ [‘Var Global’]
+  >- (gvs[eval_def,compile_exp_def,AllCaseEqs(),state_rel_def] >>
+      first_x_assum drule >>
+      rw[] >> rw[eval_def,wordLangTheory.word_op_def])
+  >~ [‘Struct’]
+  >- (gvs[eval_def,compile_exp_def,AllCaseEqs()] >>
+      simp[OPT_MMAP_MAP_o] >>
+      irule EQ_TRANS >>
+      first_assum $ irule_at $ Pos last >>
+      irule OPT_MMAP_CONG >>
+      rw[] >>
+      first_x_assum $ drule_then drule >>
+      drule_all pan_commonPropsTheory.opt_mmap_mem_func >>
+      strip_tac >> gvs[])
+  >~ [‘Load’]
+  >- (cheat (* memory *)
+     )
+  >~ [‘LoadByte’]
+  >- (cheat (* memory *)
+     )
+  >~ [‘Op’]
+  >- (gvs[eval_def,compile_exp_def,AllCaseEqs()] >>
+      first_assum $ irule_at $ Pos last >>
+      simp[OPT_MMAP_MAP_o] >>
+      irule EQ_TRANS >>
+      first_assum $ irule_at $ Pos last >>
+      irule OPT_MMAP_CONG >>
+      rw[] >>
+      first_x_assum $ drule_then drule >>
+      drule_all pan_commonPropsTheory.opt_mmap_mem_func >>
+      strip_tac >> gvs[])
+  >~ [‘Panop’]
+  >- (gvs[eval_def,compile_exp_def,AllCaseEqs()] >>
+      first_assum $ irule_at $ Pos last >>
+      simp[OPT_MMAP_MAP_o] >>
+      irule EQ_TRANS >>
+      first_assum $ irule_at $ Pos last >>
+      irule OPT_MMAP_CONG >>
+      rw[] >>
+      first_x_assum $ drule_then drule >>
+      drule_all pan_commonPropsTheory.opt_mmap_mem_func >>
+      strip_tac >> gvs[]) >>
+  gvs[wordLangTheory.word_op_def,state_rel_def,eval_def,compile_exp_def,AllCaseEqs()]
+QED
+
 Theorem resort_decls_evaluate:
   ∀s decs. evaluate_decls s (resort_decls decs) = evaluate_decls s decs
 Proof
